\documentclass{article}
\usepackage[utf8]{inputenc}
\usepackage{geometry, amsmath}
\geometry{left=2cm,right=2cm,top=2cm,bottom=2cm}
\begin{document}
\begin{align*}
P(x; \mu, \sigma^2)&=\frac{1}{\sqrt{2\pi\sigma^2}}e^{-\frac{(x-\mu)^2}{2\sigma^2}}\\
&=\frac{1}{\sqrt{2\pi}}\frac{1}{\sigma}e^{-\frac{(x-\mu)^2}{2\sigma^2}}\\
&=\frac{1}{\sqrt{2\pi}}e^{ln{\frac{1}{\sigma}}}e^{-\frac{(x-\mu)^2}{2\sigma^2}}\\
&=\frac{1}{\sqrt{2\pi}}e^{-ln(\sigma)-\frac{(x-\mu)^2}{2\sigma^2}}\\
&=\frac{1}{\sqrt{2\pi}}e^{-\frac{x^2}{2\sigma^2}+\frac{\mu x}{\sigma^2}-\frac{\mu^2}{2\sigma^2}+ln(\frac{1}{\sigma})}\\
&=\frac{1}{\sqrt{2\pi}}e^{[
\frac{\mu}{\sigma^2}\quad-\frac{1}{2\sigma^2}]
[x\quad x^2]^T-\left(\frac{\mu^2}{2\sigma^2}+ln\sigma\right)}\\
\end{align*}

For
\begin{equation}\label{final_form}
  P(x; \mu, \sigma^2)= \frac{1}{\sqrt{2\pi}}e^{[
\frac{\mu}{\sigma^2}\quad-\frac{1}{2\sigma^2}]
[x\quad x^2]^T-\left(\frac{\mu^2}{2\sigma^2}+ln\sigma\right)}
\end{equation}

In Eq~\ref{final_form}, counting measure is $1/\sqrt{2\pi}$, natural parameter $\eta$ is $[
\frac{\mu}{\sigma^2}\quad-\frac{1}{2\sigma^2}]$, sufficient statistics $t(x)$ are $[x\quad x^2]$, $a(\eta)$ is $\left(\frac{\mu^2}{2\sigma^2}+ln\sigma\right)$.

\begin{align*}
    \eta_1&=\frac{\mu}{\sigma^2}\\
    \eta_2&=-\frac{1}{2\sigma^2}
\end{align*}

Thus, 
$$
\mu=\frac{\eta_1}{-2\eta_2}
$$

And,

\begin{align*}
a(\eta)&=\left[\frac{(\frac{\eta_1}{2\eta_2})^2}{2(\frac{1}{-2\eta_2})^2}+ln\sqrt{\frac{1}{-2\eta_2}}\right]=-\frac{1}{2}\eta_1^2\frac{1}{2\eta_2}-\frac{1}{2}ln(-2\eta_2)\\
&=\frac{\eta_1^2}{4\eta_2}-\frac{1}{2}ln(-2\eta_2)\\
\end{align*}

\end{document}
